Proved assume in matrix_mul; cleanup

frodo/code/Hacl.Impl.PQ.Lib.fst
@@ -105,8 +105,6 @@ val map2_inner_inv:
   -> Type0
 let map2_inner_inv #n1 #n2 h0 h1 h2 f a b c i j =
   B.live h2 a /\ B.live h2 b /\ B.live h2 c /\
-  a == c /\
-  B.disjoint b c /\
   modifies (loc_buffer c) h1 h2 /\
   j <= v n2 /\
   (forall (i0:nat{i0 < v i}) (j:nat{j < v n2}). get h2 c i0 j == get h1 c i0 j) /\
@@ -123,7 +121,7 @@ val map2_inner:
   -> f:(elem -> elem -> elem)
   -> a:matrix_t n1 n2
   -> b:matrix_t n1 n2
-  -> c:matrix_t n1 n2
+  -> c:matrix_t n1 n2{a == c /\ B.disjoint b c}
   -> i:size_t{v i < v n1}
   -> j:size_t{v j < v n2}
   -> Stack unit
@@ -146,10 +144,11 @@ val map2:
   -> b:matrix_t n1 n2
   -> c:matrix_t n1 n2
   -> Stack unit
-    (requires fun h0 -> B.live h0 a /\ B.live h0 b /\ B.live h0 c /\ a == c /\ B.disjoint b c)
+    (requires fun h0 -> 
+      B.live h0 a /\ B.live h0 b /\ B.live h0 c /\ a == c /\ B.disjoint b c)
     (ensures  fun h0 _ h1 ->
       modifies (loc_buffer c) h0 h1 /\
-      as_matrix h1 c == M.map2 #(v n1) #(v n2) f (as_matrix h0 a) (as_matrix h0 b) )
+      as_matrix h1 c == M.map2 #(v n1) #(v n2) f (as_matrix h0 a) (as_matrix h0 b))
 let map2 #n1 #n2 f a b c =
   let h0 = ST.get () in
   Lib.Loops.for (size 0) n1
@@ -203,6 +202,8 @@ let matrix_sub #n1 #n2 a b =
   let h1 = ST.get() in
   M.extensionality (as_matrix h1 b) (M.sub (as_matrix h0 a) (as_matrix h0 b))
 
+#reset-options "--z3rlimit 50 --max_fuel 1 --max_ifuel 0"
+
 inline_for_extraction noextract private
 val mul_inner:
     #n1:size_t
@@ -213,42 +214,42 @@ val mul_inner:
   -> i:size_t{v i < v n1}
   -> k:size_t{v k < v n3}
   -> Stack uint16
-    (requires (fun h -> B.live h a /\ B.live h b))
-    (ensures (fun h0 r h1 -> modifies loc_none h0 h1 /\
-      r == M.mul_inner #(v n1) #(v n2) #(v n3) (as_matrix h0 a) (as_matrix h0 b) (v i) (v k)))
-#reset-options "--z3rlimit 50 --max_fuel 1"
+    (requires fun h -> B.live h a /\ B.live h b)
+    (ensures  fun h0 r h1 -> 
+      modifies loc_none h0 h1 /\
+      r == M.mul_inner (as_matrix h0 a) (as_matrix h0 b) (v i) (v k))
 let mul_inner #n1 #n2 #n3 a b i k =
   push_frame();
   let h0 = ST.get() in
-  [@ inline_let ]
-  let f = (fun l -> get h0 a (v i) l *. get h0 b l (v k)) in
-  [@ inline_let ]
-  let f1 (j:size_nat{j <= v n2}) = M.sum_ #(v n2) f j in
-  let res:lbuffer uint16 1 = create (size 1) (u16 0) in
+  let f l = get h0 a (v i) l *. get h0 b l (v k) in
+  let f1 j = M.sum_ #(v n2) f j in
+  let res = create #uint16 #1 (size 1) (u16 0) in
   let h1 = ST.get() in
-
-  let inv (h2: HS.mem) (i:nat{i <= v n2}): Type0 =
+  let inv h2 (i:nat{i <= v n2}) =
     B.live h1 res /\ B.live h2 res /\
     modifies (loc_buffer res) h1 h2 /\
     B.get h2 res 0 == f1 i in
-  let f' (j:size_t{ 0 <= v j /\ v j < v n2}): Stack unit
-    (requires (fun h -> inv h (v j)))
-    (ensures (fun h_1 _ h_2 -> inv h_2 (v j + 1)))
+  let f' (j:size_t{0 <= v j /\ v j < v n2}) : Stack unit
+    (requires fun h -> inv h (v j))
+    (ensures  fun _ _ h2 -> inv h2 (v j + 1))
   =
-    let aij = mget a i j in
-    let bjk = mget b j k in
-    let res0 = res.(size 0) in
-    res.(size 0) <- res0 +. aij *. bjk in
+    let aij = a.[i,j] in
+    let bjk = b.[j,k] in
+    let res0 = !*res in
+    res *= (res0 +. aij *. bjk)
+  in
   Lib.Loops.for (size 0) n2 inv f';
-  let res = res.(size 0) in
+  let res = !*res in
   M.sum_extensionality (v n2) f (fun l -> get h0 a (v i) l *. get h0 b l (v k)) (v n2);
-  assert (res == M.mul_inner #(v n1) #(v n2) #(v n3) (as_matrix h0 a) (as_matrix h0 b) (v i) (v k));
+  assert (res == M.mul_inner (as_matrix h0 a) (as_matrix h0 b) (v i) (v k));
   pop_frame();
   res
 
+#reset-options "--z3rlimit 50 --max_fuel 0 --max_ifuel 0"
+
 private unfold
 val mul_inner_inv:
-  #n1:size_t
+    #n1:size_t
   -> #n2:size_t{v n1 * v n2 < max_size_t}
   -> #n3:size_t{v n2 * v n3 < max_size_t /\ v n1 * v n3 < max_size_t}
   -> h0:HS.mem
@@ -257,44 +258,52 @@ val mul_inner_inv:
   -> a:matrix_t n1 n2
   -> b:matrix_t n2 n3
   -> c:matrix_t n1 n3
-  -> f:(k:size_nat{k < v n3} -> GTot uint16)
+  -> f:(k:nat{k < v n3} -> GTot uint16)
   -> i:size_t{v i < v n1}
   -> k:size_nat
   -> Type0
 let mul_inner_inv #n1 #n2 #n3 h0 h1 h2 a b c f i k =
   B.live h2 a /\ B.live h2 b /\ B.live h2 c /\
-  B.disjoint a c /\ B.disjoint b c /\
   modifies (loc_buffer c) h1 h2 /\
   k <= v n3 /\
-  (forall (i1:size_nat{i1 < v i}) (k:size_nat{k < v n3}). get h2 c i1 k == get h1 c i1 k) /\
-  (forall (k1:size_nat{k1 < k}). get h2 c (v i) k1 == f k1) /\
-  (forall (k1:size_nat{k <= k1 /\ k1 < v n3}). get h2 c (v i) k1 == get h0 c (v i) k1) /\
-  (forall (i1:size_nat{v i < i1 /\ i1 < v n1}) (k:size_nat{k < v n3}). get h2 c i1 k == get h0 c i1 k) /\
-  as_matrix h0 a == as_matrix h2 a /\
+  (forall (i1:nat{i1 < v i}) (k:nat{k < v n3}). get h2 c i1 k == get h1 c i1 k) /\
+  (forall (k1:nat{k1 < k}). get h2 c (v i) k1 == f k1) /\
+  (forall (k1:nat{k <= k1 /\ k1 < v n3}). get h2 c (v i) k1 == get h0 c (v i) k1) /\
+  (forall (i1:nat{v i < i1 /\ i1 < v n1}) (k:nat{k < v n3}). get h2 c i1 k == get h0 c i1 k) /\
+  as_matrix h0 a == as_matrix h2 a /\ 
   as_matrix h0 b == as_matrix h2 b
 
 inline_for_extraction noextract private
 val mul_inner1:
-  #n1:size_t
+    #n1:size_t
   -> #n2:size_t{v n1 * v n2 < max_size_t}
   -> #n3:size_t{v n2 * v n3 < max_size_t /\ v n1 * v n3 < max_size_t}
   -> h0:HS.mem
   -> h1:HS.mem
   -> a:matrix_t n1 n2
   -> b:matrix_t n2 n3
-  -> c:matrix_t n1 n3
+  -> c:matrix_t n1 n3{B.disjoint a c /\ B.disjoint b c}
   -> i:size_t{v i < v n1}
   -> k:size_t{v k < v n3}
-  -> f:(k:size_nat{k < v n3} -> GTot (res:uint16{res == M.sum #(v n2) (fun l -> get h0 a (v i) l *. get h0 b l k)}))
+  -> f:(k:nat{k < v n3} 
+       -> GTot (res:uint16{res == M.sum #(v n2) (fun l -> get h0 a (v i) l *. get h0 b l k)}))
   -> Stack unit
-    (requires fun h2 -> mul_inner_inv #n1 #n2 #n3 h0 h1 h2 a b c f i (v k))
-    (ensures  fun _ _ h2 -> mul_inner_inv #n1 #n2 #n3 h0 h1 h2 a b c f i (v k + 1))
+    (requires fun h2 -> mul_inner_inv h0 h1 h2 a b c f i (v k))
+    (ensures  fun _ _ h2 -> mul_inner_inv h0 h1 h2 a b c f i (v k + 1))
 let mul_inner1 #n1 #n2 #n3 h0 h1 a b c i k f =
-  assert (M.mul_inner #(v n1) #(v n2) #(v n3) (as_matrix h0 a) (as_matrix h0 b) (v i) (v k) ==
+  assert (M.mul_inner (as_matrix h0 a) (as_matrix h0 b) (v i) (v k) ==
           M.sum #(v n2) (fun l -> get h0 a (v i) l *. get h0 b l (v k)));
-  mset c i k (mul_inner #n1 #n2 #n3 a b i k);
+  c.[i,k] <- mul_inner a b i k;
   let h2 = ST.get () in
   assert (get h2 c (v i) (v k) == f (v k))
+
+#reset-options "--z3rlimit 50 --max_fuel 1 --max_ifuel 1"
+
+private
+val onemore: p:(nat -> Type0) -> q:(i:nat{p i} -> Type0) -> b:nat{p b} -> Lemma
+  (requires (forall (i:nat{p i /\ i < b}). q i) /\ q b)
+  (ensures  forall (i:nat{p i /\ i <= b}). q i)
+let onemore p q b = ()
 
 val matrix_mul:
     #n1:size_t
@@ -304,70 +313,70 @@ val matrix_mul:
   -> b:matrix_t n2 n3
   -> c:matrix_t n1 n3
   -> Stack unit
-    (requires (fun h -> B.live h a /\ B.live h b /\ B.live h c /\
-      B.disjoint a c /\ B.disjoint b c))
-    (ensures (fun h0 _ h1 -> B.live h1 c /\ modifies (loc_buffer c) h0 h1 /\
-      as_matrix h1 c == M.mul #(v n1) #(v n2) #(v n3) (as_matrix h0 a) (as_matrix h0 b)))
-#reset-options "--z3rlimit 50 --max_fuel 1"
+    (requires fun h -> 
+      B.live h a /\ B.live h b /\ B.live h c /\ B.disjoint a c /\ B.disjoint b c)
+    (ensures  fun h0 _ h1 -> 
+      B.live h1 c /\ 
+      modifies (loc_buffer c) h0 h1 /\
+      as_matrix h1 c == M.mul (as_matrix h0 a) (as_matrix h0 b))
 [@"c_inline"]
 let matrix_mul #n1 #n2 #n3 a b c =
   let h0 = ST.get () in
-  [@ inline_let ]
-  let f (i:size_nat{i < v n1}):
-    (k:size_nat{k < v n3} -> GTot (res:uint16{res == M.sum #(v n2) (fun l -> get h0 a i l *. get h0 b l k)}))
-  = fun k -> M.sum #(v n2) (fun l -> get h0 a i l *. get h0 b l k) in
-
+  let f (i:nat{i < v n1}) (k:nat{k < v n3}) : 
+    GTot (res:uint16{res == M.sum #(v n2) (fun l -> get h0 a i l *. get h0 b l k)})
+  = M.sum #(v n2) (fun l -> get h0 a i l *. get h0 b l k) 
+  in
   Lib.Loops.for (size 0) n1
-    (fun h1 i -> B.live h1 a /\ B.live h1 b /\ B.live h1 c /\
+    (fun h1 i -> 
+      B.live h1 a /\ B.live h1 b /\ B.live h1 c /\
       modifies (loc_buffer c) h0 h1 /\ i <= v n1 /\
       (forall (i1:nat{i1 < i}) (k:nat{k < v n3}). get h1 c i1 k == f i1 k) /\
       (forall (i1:nat{i <= i1 /\ i1 < v n1}) (k:nat{k < v n3}). get h1 c i1 k == get h0 c i1 k))
     (fun i ->
       let h1 = ST.get() in
-      [@ inline_let ]
-      let f1 = f (v i) in
       Lib.Loops.for (size 0) n3
-        (fun h2 k -> mul_inner_inv #n1 #n2 #n3 h0 h1 h2 a b c f1 i k)
-        (fun k -> mul_inner1 #n1 #n2 #n3 h0 h1 a b c i k f1);
-      let h1 = ST.get () in
-      assert (forall (i1:nat{i1 < v i}) (k:nat{k < v n3}). get h1 c i1 k == f i1 k);
-      assert (forall (k:nat{k < v n3}). get h1 c (v i) k == f (v i) k);
-      assume (forall (i1:nat{i1 < v i + 1}) (k:nat{k < v n3}). get h1 c i1 k == f i1 k) //FIXME
+        (fun h2 k -> mul_inner_inv h0 h1 h2 a b c (f (v i)) i k)
+        (fun k -> mul_inner1 h0 h1 a b c i k (f (v i)));
+      let h1 = ST.get() in
+      let q i1 = forall k. get h1 c i1 k == f i1 k in      
+      onemore (fun i1 -> i1 < v n1) q (v i)
     );
   let h2 = ST.get() in
-  M.extensionality (as_matrix h2 c) (M.mul #(v n1) #(v n2) #(v n3) (as_matrix h0 a) (as_matrix h0 b))
+  M.extensionality (as_matrix h2 c) (M.mul (as_matrix h0 a) (as_matrix h0 b))
+
 
 val eq_u32_m:m:uint32 -> a:uint32 -> b:uint32 -> Tot bool
 [@ "substitute"]
 let eq_u32_m m a b =
   let open Lib.RawIntTypes in
-  FStar.UInt32.(u32_to_UInt32 (a &. m) =^ u32_to_UInt32 (b &. m))
+  let open FStar.UInt32 in
+  u32_to_UInt32 (a &. m) =^ u32_to_UInt32 (b &. m)
 
 val matrix_eq:
-  #n1:size_t
+    #n1:size_t
   -> #n2:size_t{v n1 * v n2 < max_size_t}
   -> m:size_t{0 < v m /\ v m <= 16}
   -> a:matrix_t n1 n2
   -> b:matrix_t n1 n2
   -> Stack bool
-    (requires (fun h -> B.live h a /\ B.live h b))
-    (ensures (fun h0 r h1 -> modifies loc_none h0 h1))
+    (requires fun h -> B.live h a /\ B.live h b)
+    (ensures  fun h0 r h1 -> modifies loc_none h0 h1)
 [@"c_inline"]
 let matrix_eq #n1 #n2 m a b =
   push_frame();
   let m = (u32 1 <<. size_to_uint32 m) -. u32 1 in
-  let res:lbuffer bool 1 = create (size 1) true in
-  let h0 = ST.get () in
-  loop_nospec #h0 n1 res
+  let res = create #bool #1 (size 1) true in
+  let h0 = ST.get() in
+  loop_nospec #h0 #bool #1 n1 res
   (fun i ->
-    let h1 = ST.get () in
-    loop_nospec #h1 n2 res
+    let h1 = ST.get() in
+    loop_nospec #h1 #bool #1 n2 res
     (fun j ->
-      let a1 = res.(size 0) in
+      let a1 = !*res in
       let a2 = eq_u32_m m (to_u32 (mget a i j)) (to_u32 (mget b i j)) in
-      res.(size 0) <- a1 && a2
+      res *= (a1 && a2)
     )
   );
-  let res = res.(size 0) in
+  let res = !*res in
   pop_frame();
   res
